Simu/Tra.v
@@ -45,8 +45,7 @@ Definition translate_const (c: const): typ -> Clight.expr :=
 Definition translate_exp (cls: ident) (e: exp): Clight.expr :=
   match e with
   | Var x ty => Clight.Evar x ty  
-  | State x ty =>
-    deref_self_field cls x ty
+  | State x ty => deref_self_field cls x ty
   | Const c ty => translate_const c ty
   end.
 
@@ -56,20 +55,18 @@ Fixpoint list_type_to_typelist (tys: list typ): Ctypes.typelist :=
   | ty :: tys => Ctypes.Tcons ty (list_type_to_typelist tys)
   end.
 
-Definition funcall
-           (bind: option ident) (f: ident) (ty: typ) (args: list Clight.expr)
-  : Clight.statement :=
+Definition funcall (f: ident) (args: list Clight.expr) : Clight.statement :=
   let tys := List.map Clight.typeof args in
-  let sig := Ctypes.Tfunction (list_type_to_typelist tys) ty AST.cc_default in
-  Clight.Scall bind (Clight.Evar f sig) args.
+  let sig := Ctypes.Tfunction (list_type_to_typelist tys) Ctypes.Tvoid AST.cc_default in
+  Clight.Scall None (Clight.Evar f sig) args.
 
-Definition assign (bind: ident) (ty: typ) (e: Clight.expr): Clight.statement :=
-  Clight.Sassign (Clight.Evar bind ty) e.
+Definition assign (x: ident) (ty: typ) (e: Clight.expr): Clight.statement :=
+  Clight.Sassign (Clight.Evar x ty) e.
 
-Definition binded_funcall (bind temp f: ident) (ty: typ) (args: list Clight.expr)
-  : Clight.statement :=
-   Clight.Ssequence (funcall (Some temp) f ty args)
-                   (assign bind ty (Clight.Etempvar temp ty)).
+(* Definition binded_funcall (bind temp f: ident) (ty: typ) (args: list Clight.expr) *)
+(*   : Clight.statement := *)
+(*    Clight.Ssequence (funcall (Some temp) f ty args) *)
+(*                     (assign bind ty (Clight.Etempvar temp ty)). *)
 
 Definition ptr_obj (owner: option ident) (cls obj: ident): Clight.expr :=
   Clight.Eaddrof
@@ -79,62 +76,63 @@ Definition ptr_obj (owner: option ident) (cls obj: ident): Clight.expr :=
       end) obj (type_of_inst cls))
     (type_of_inst_p cls).
 
-Definition step_call
-           (owner: option ident) (bind temp cls: ident) (obj: ident) (args: list Clight.expr)
-           (out_ty: typ)
+Definition step_call (owner: option ident) (cls obj: ident) (args: list Clight.expr)
   : Clight.statement :=
   let args := ptr_obj owner cls obj :: args in
-  binded_funcall bind temp (step_id cls) out_ty args.
+  funcall (step_id cls) args.
+
+Definition make_in_arg (arg: ident * typ): Clight.expr :=
+  let (x, ty) := arg in
+  Clight.Evar x ty.
+Definition make_out_arg (arg: ident * typ): Clight.expr :=
+  let (x, ty) := arg in
+  Clight.Eaddrof (Clight.Evar x ty) (pointer_of ty).
+
 (** 
 Statement conversion keeps track of the produced temporaries (function calls).
 [owner] represents the name of the current class.
  *)
-Fixpoint translate_stmt (temp: option (ident * typ)) (owner: ident) (s: stmt)
-  : option (ident * typ) * Clight.statement :=
+Fixpoint translate_stmt (owner: ident) (s: stmt): Clight.statement :=
   match s with
   | Assign x e =>
-    (temp, Clight.Sassign (Clight.Evar x (typeof e)) (translate_exp owner e))
+    Clight.Sassign (Clight.Evar x (typeof e)) (translate_exp owner e)
   | AssignSt x e =>
-    (temp, Clight.Sassign (deref_self_field owner x (typeof e)) (translate_exp owner e))
+    Clight.Sassign (deref_self_field owner x (typeof e)) (translate_exp owner e)
   | Ifte e s1 s2 =>
-    let (temp1, s1') := translate_stmt temp owner s1 in
-    let (temp2, s2') := translate_stmt temp1 owner s2 in
-    (temp2, Clight.Sifthenelse (translate_exp owner e) s1' s2')
+    Clight.Sifthenelse (translate_exp owner e)
+                       (translate_stmt owner s1) (translate_stmt owner s2)
   | Comp s1 s2 =>
-    let (temp1, s1') := translate_stmt temp owner s1 in
-    let (temp2, s2') := translate_stmt temp1 owner s2 in
-    (temp2, Clight.Ssequence s1' s2')
-  | Step_ap y ty cls x es =>
+    Clight.Ssequence (translate_stmt owner s1) (translate_stmt owner s2)
+  | Step_ap ys cls x es =>
     let args := nelist2list (Nelist.map (translate_exp owner) es) in
-    let temp' := match temp with Some t => t | None => (first_unused_ident tt, ty) end in
-    let s_step := step_call (Some owner) y (fst temp') cls x args ty in 
-    (Some temp', s_step)
+    let outs := nelist2list (Nelist.map make_out_arg ys) in
+    step_call (Some owner) cls x (args ++ outs)  
   | Skip =>
-    (temp, Clight.Sskip)
+    Clight.Sskip
   end.
 
-
-Definition return_some (s: Clight.statement) (out: ident * typ): Clight.statement :=
-  let (id, ty) := out in
-  Clight.Ssequence s (Clight.Sreturn (Some (Clight.Evar id ty))).
+(* Definition return_some (s: Clight.statement) (out: ident * typ): Clight.statement := *)
+(*   let (id, ty) := out in *)
+(*   Clight.Ssequence s (Clight.Sreturn (Some (Clight.Evar id ty))). *)
+Definition return_none (s: Clight.statement): Clight.statement :=
+  Clight.Ssequence s (Clight.Sreturn None).
 Definition cl_zero: Clight.expr :=
   Clight.Econst_int Int.zero Ctypes.type_int32s.
 Definition return_zero (s: Clight.statement): Clight.statement :=
   Clight.Ssequence s (Clight.Sreturn (Some cl_zero)).
 
 Definition fundef
-           (ins: list (ident * typ)) (vars: list (ident * typ)) (ty: typ)
-           (temps: list (ident * typ)) (body: Clight.statement)
+           (ins: list (ident * typ)) (vars: list (ident * typ)) (ty: typ) (body: Clight.statement)
   : AST.globdef Clight.fundef Ctypes.type :=
-  let f := Clight.mkfunction ty AST.cc_default ins vars temps body in
-  @AST.Gfun Clight.fundef typ (Clight.Internal f).
+  let f := Clight.mkfunction ty AST.cc_default ins vars [] body in
+  @AST.Gfun Clight.fundef typ (Ctypes.Internal f).
 
 Definition make_step
-           (self: ident * typ) (ins: list (ident * typ)) (out: ident * typ)
-           (vars: list (ident * typ)) (temps: list (ident * typ)) (body: Clight.statement)
+           (self: ident * typ) (ins: list (ident * typ)) (outs: list (ident * typ))
+           (vars: list (ident * typ)) (body: Clight.statement)
   : AST.globdef Clight.fundef Ctypes.type :=
-  let body := return_some body out in
-  fundef (self :: ins) vars (snd out) temps body.
+  let body := return_none body in
+  fundef (self :: ins ++ outs) vars Ctypes.Tvoid body.
 
 Definition translate_obj_dec (obj: obj_dec): (ident * typ) :=
   match obj with
@@ -152,11 +150,10 @@ Definition translate_class (c: class)
     mk_class c_name c_input c_output c_vars c_mems c_objs c_step =>
     let objs := List.map translate_obj_dec c_objs in
     let members := c_mems ++ objs in
-    let (temp_step, step) := translate_stmt None c_name c_step in
+    let step := translate_stmt c_name c_step in
     let self := (self_id, type_of_inst_p c_name) in
-    let temp_step' := match temp_step with Some t => [t] | None => [] end in
     let cl_struct := make_struct c_name members in
-    let cl_step := (step_id c_name, make_step self (nelist2list c_input) c_output c_vars temp_step' step) in
+    let cl_step := (step_id c_name, make_step self (nelist2list c_input) (nelist2list c_output) c_vars step) in
     (cl_struct, cl_step)
   end.
 
@@ -165,18 +162,15 @@ Definition glob_id (id: ident): ident :=
 Definition glob_bind (bind: ident * typ): ident * typ :=
   let (x, ty) := bind in
   (glob_id x, ty).
-Definition make_arg (arg: ident * typ): Clight.expr :=
-  let (x, ty) := arg in
-  Clight.Evar (glob_id x) ty.
 
-Definition make_main (node: ident) (f: ident) (ins: list (ident * typ)) (out: ident * typ)
+Definition make_main (node: ident) (f: ident) (ins: list (ident * typ)) (outs: list (ident * typ))
   : AST.globdef Clight.fundef Ctypes.type :=
-  let (out, out_ty) := out in
-  let args := List.map make_arg ins in
-  let step := step_call None out out node f args out_ty in
+  let args_in := List.map make_in_arg ins in
+  let args_out := List.map make_out_arg outs in
+  let step := step_call None node f (args_in ++ args_out) in
   let loop := Clight.Sloop ((* Clight.Ssequence wait *) step) Clight.Sskip in
   let body := return_zero ((* Clight.Ssequence (reset_call None node f) *) loop) in
-  fundef [] [] Ctypes.type_int32s [(out, out_ty)] body.
+  fundef [] [] Ctypes.type_int32s body.
 
 Definition vardef (init volatile: bool) (x: ident * typ): ident * AST.globdef Clight.fundef Ctypes.type :=
   let (x, ty) := x in
@@ -184,21 +178,19 @@ Definition vardef (init volatile: bool) (x: ident * typ): ident * AST.globdef Cl
   (x, @AST.Gvar Clight.fundef _
                 (AST.mkglobvar ty' (if init then [AST.Init_space Z0] else []) false volatile)).
 
-Definition translate (p: program) (main_node: ident)
-  : Errors.res Clight.program :=
+Definition translate (p: program) (main_node: ident): Errors.res Clight.program :=
   match find_class main_node p with
   | Some (cls, _) =>
     let f := glob_id main_node in
-    let ins := nelist2list cls.(c_input) in
-    let out' := glob_bind cls.(c_output) in
-    let main := make_main main_node f ins out' in
+    let ins := map glob_bind (nelist2list cls.(c_input)) in
+    let outs := map glob_bind (nelist2list cls.(c_output)) in
+    let main := make_main main_node f ins outs in
     let cs := List.map translate_class p in
     let f_gvar := vardef true false (f, type_of_inst main_node) in
-    let o_gvar := vardef true true out' in
-    let ins' := List.map glob_bind ins in
-    let ins_gvar := List.map (vardef true true) ins' in
+    let o_gvars := map (vardef true true) outs in
+    let i_gvars := map (vardef true true) ins in
     let (structs, steps) := split cs in
-    let gdefs := f_gvar :: o_gvar :: ins_gvar ++ steps ++ [(main_id, main)] in
-    Clight.make_program structs gdefs [] main_id                    
+    let gdefs := f_gvar :: o_gvars ++ i_gvars ++ steps ++ [(main_id, main)] in
+    Ctypes.make_program structs gdefs [] main_id                    
   | None => Errors.Error (Errors.msg "undefined node")
   end.
